LLVM_DS_RBT/Insert/Alloc_Optimized/Insert_Opt_Ext.thy
@@ -12,11 +12,11 @@ begin
 lemma pure_assn_prem_from_prem: "(P1 \<Longrightarrow> P2 \<Longrightarrow> htriple P3 c Q) \<Longrightarrow> htriple (\<up>P1 ** \<up>P2 ** P3) c Q"
   by (metis (mono_tags) htriple_realizable_preI n1 pure_true_conv realizable_extract_pure)
 
-lemma less_key_not_in_value_graph [dest]: "(k, vi) \<in> at_value_graph t ti \<Longrightarrow> (rbt_of t) |\<guillemotleft> k \<Longrightarrow> False"
-  apply (induction t arbitrary: ti) by auto
+lemma less_key_not_in_value_graph [dest]: "(k, vi) \<in> at_value_graph t \<Longrightarrow> (rbt_of t) |\<guillemotleft> k \<Longrightarrow> False"
+  apply (induction t) by auto
 
-lemma greater_key_not_in_value_graph [dest]: "(k, vi) \<in> at_value_graph t ti \<Longrightarrow> k \<guillemotleft>| (rbt_of t) \<Longrightarrow> False"
-  apply (induction t arbitrary: ti) by auto
+lemma greater_key_not_in_value_graph [dest]: "(k, vi) \<in> at_value_graph t \<Longrightarrow> k \<guillemotleft>| (rbt_of t) \<Longrightarrow> False"
+  apply (induction t) by auto
 
 lemma insert'_opt_correct_ext:
   "
@@ -27,7 +27,7 @@ lemma insert'_opt_correct_ext:
       \<up>(rbt_of res_t = (rbt_ins (\<lambda>_ _ v. v)) k v (rbt_of t)) **
       \<up>(rbt_sorted (rbt_of res_t)) **
       \<up>(ptr_of_key t ti \<subseteq>\<^sub>m ptr_of_key res_t res) **
-      \<up>(value_of_key res_t res = (value_of_key t ti)(k \<mapsto> vi))
+      \<up>(value_of_key res_t = (value_of_key t)(k \<mapsto> vi))
     )
   "
   supply ptr_of_key_subsetD[dest!]
@@ -39,7 +39,7 @@ proof (induction k v "rbt_of t" arbitrary: t ti rule: rbt_insert_ad'.induct )
     apply vcg
     apply vcg_compat
     apply (sepEwith \<open>vok_filter,auto?\<close>)
-    apply simp
+     apply vok_solver
     apply (sepwith simp)
     done
 next
@@ -53,7 +53,7 @@ next
                    \<up>(rbt_of x = rbt_ins (\<lambda>_ _ v. v) k\<^sub>n v\<^sub>n (rbt_of t)) \<and>*
                    \<up>rbt_sorted (rbt_of x) \<and>*
                    \<up>(ptr_of_key t ti \<subseteq>\<^sub>m ptr_of_key x res) \<and>*
-                   \<up>(value_of_key x res = value_of_key t ti(k\<^sub>n \<mapsto> vi)))
+                   \<up>(value_of_key x = value_of_key t(k\<^sub>n \<mapsto> vi)))
                    s)" for t ti supply 2(1)[vcg_rules] by vcg
 
   have []:
@@ -64,7 +64,7 @@ next
                    \<up>(rbt_of x = rbt_ins (\<lambda>_ _ v. v) k\<^sub>n v\<^sub>n (rbt_of t)) \<and>*
                    \<up>rbt_sorted (rbt_of x) \<and>*
                    \<up>(ptr_of_key t ti \<subseteq>\<^sub>m ptr_of_key x res) \<and>*
-                   \<up>(value_of_key x res = value_of_key t ti(k\<^sub>n \<mapsto> vi)))
+                   \<up>(value_of_key x = value_of_key t (k\<^sub>n \<mapsto> vi)))
                    s)" for t ti supply 2(2)[vcg_rules] by vcg
 
   from 2(3) show ?case
@@ -75,10 +75,10 @@ next
     supply 
       rbt_greater_trans[intro]
       rbt_less_trans[intro]      
-      value_of_key_simps[simp]
+      value_of_key'_simps[simp]
 
     supply 2(1-2)[vcg_rules] 
-    apply (vcg;fail) 
+    apply (vcg;fail)
     done
 next
   case (3 k\<^sub>n v\<^sub>n l k v r)
@@ -92,7 +92,7 @@ next
     supply 
       rbt_greater_trans[intro]
       rbt_less_trans[intro]      
-      value_of_key_simps[simp]
+      value_of_key'_simps[simp]
     apply (vcg;fail)
     done
 qed
@@ -107,7 +107,7 @@ lemma insert_opt_correct_ext' [vcg_rules]:
       \<up>(rbt_of res_t = rbt_insert k v (rbt_of t)) **
       \<up>(rbt_sorted (rbt_of res_t)) **
       \<up>(ptr_of_key t ti \<subseteq>\<^sub>m ptr_of_key res_t res_ti) **
-      \<up>(value_of_key res_t res_ti = (value_of_key t ti)(k \<mapsto> vi))
+      \<up>(value_of_key res_t = (value_of_key t)(k \<mapsto> vi))
     )
   "
   unfolding insert_opt_def rbt_insert_def rbt_insert_with_key_def paint_def
@@ -119,10 +119,10 @@ lemma insert_opt_correct_ext' [vcg_rules]:
   apply (subgoal_tac "rbt_sorted (rbt_of (ATBranch color.B x23 x24 1 li ki vi ri al ar))")
    apply vcg_compat 
    apply (sepEwith \<open>auto dest!: ptr_of_key_subsetD\<close>)
-    apply (auto simp add: value_of_key_simps intro: rbt_less_trans rbt_greater_trans)[]  
+    apply (auto simp add: value_of_key'_simps intro: rbt_less_trans rbt_greater_trans)[]  
   apply simp
-  using ins_rbt_sorted rbt_of.simps(2) rbt_sorted.simps(2) 
-  by metis 
+  using ins_rbt_sorted rbt_of.simps(2) rbt_sorted.simps(2)
+  by metis
  
   
 
@@ -137,7 +137,7 @@ lemma insert_opt_correct_ext [vcg_rules]:
       \<up>(rbt_of res_t = rbt_insert k v (rbt_of t)) **
       \<up>(is_rbt (rbt_of res_t)) **
       \<up>(ptr_of_key t ti \<subseteq>\<^sub>m ptr_of_key res_t res_ti) **
-      \<up>(value_of_key res_t res_ti = (value_of_key t ti)(k \<mapsto> vi))
+      \<up>(value_of_key res_t = (value_of_key t)(k \<mapsto> vi))
     )
   "
   apply vcg
